More type-class based unified memory model
This is to overcome most, but not all, needs for explicit type
casts.

This way is also more extensible.

src/tls/Mem.fst
@@ -7,71 +7,96 @@ module MS = FStar.Monotonic.Seq
 
 let mem = HS.mem
 
-abstract
+unfold
+let grows (a: Type) (p: (Seq.seq a -> Type)) (s1 s2: (s: Seq.seq a {p s})) = MS.grows s1 s2
+
+let is_eternal_region = HS.is_eternal_region
+
 noeq
-type loc =
-| LocRef: (
-    (a: Type) ->
-    (contents: HS.reference a) ->
-    loc
- )
-| LocMRef: (
-    (r: MR.rid) ->
-    (a: Type) ->
-    (b: MR.reln a) ->
-    (contents: MR.m_rref r a b) ->
-    loc
-  )
-| LocISeq: (
-    (r: MS.rid) ->
-    (a: Type) ->
-    (p: (Seq.seq a -> Type)) ->
-    (contents: MS.i_seq r a p) ->
-    loc
-  )
+type class = | Class :
+  (ref: Type) ->
+  (value: Type) ->
+  (as_reference: (ref -> GTot (HS.reference value))) ->
+  (region_guard: (HH.rid -> GTot Type)) ->
+  (region_guarded: (
+    (r: ref) ->
+    Lemma
+    (region_guard (HS.frameOf (as_reference r)))
+  )) ->
+  (reln: MR.reln value) ->
+  (recall: (
+    (r: ref) ->
+    Stack unit
+    (requires (fun _ ->
+      let rr = as_reference r in (
+      is_eternal_region (HS.frameOf rr) /\
+      (~ rr.HS.mm)
+    )))
+    (ensures (fun m0 _ m1 ->
+      m0 == m1 /\ m1 `HS.contains` (as_reference r)
+    ))
+  )) ->
+  (read: (
+    (r: ref) ->
+    ST value
+    (requires (fun h -> HS.weak_contains h (as_reference r)))
+    (ensures (fun m0 x m1 -> m1 == m0 /\ x == HS.sel m0 (as_reference r)))
+  )) ->
+  (write_pre: (
+    (r: ref) ->
+    (v: value) ->
+    (h: mem) ->
+    GTot Type
+  )) ->
+  (write: (
+    (r: ref) ->
+    (v: value) ->
+    ST unit
+    (requires (fun h0 -> h0 `HS.contains` (as_reference r) /\ write_pre r v h0))
+    (ensures (fun m0 _ m1 ->
+      m0 `HS.contains` (as_reference r) /\
+      m1 == HS.upd m0 (as_reference r) v
+  )))) ->
+  class
 
-abstract
-let is_ref (l: loc): GTot bool = LocRef? l
+noeq
+type loc = | Loc :
+  (cl: class) ->
+  (obj: Class?.ref cl) ->
+  loc
 
-let guarded (t: Type) (p: (t -> Type)) : Tot Type = (x: t {p x})
+unfold
+let ref_cl (a: Type): Tot class = Class
+  (HS.reference a)
+  a
+  (fun x -> x)
+  (fun _ -> True)
+  (fun _ -> ())
+  (fun _ _ -> False)
+  (fun r -> ST.recall r)
+  (fun r -> !r)
+  (fun _ _ _ -> True)
+  (fun r v -> r := v)
 
-abstract
-let loc_type (l: loc) : GTot Type =
-  match l with
-  | LocRef a _ -> a
-  | LocMRef _ a _ _ -> a
-  | LocISeq _ a p _ -> guarded (Seq.seq a) p
+let ref (a: Type) : Tot Type = (l: loc { Loc?.cl l == ref_cl a } )
 
-abstract
-let loc_ref (l: loc { is_ref l } ) : GTot (HS.reference (loc_type l)) = LocRef?.contents l
+unfold
+let mref_cl (r: MR.rid) (a: Type) (b: MR.reln a) : Tot class = Class
+  (MR.m_rref r a b)
+  a
+  (MR.as_hsref #r #a #b)
+  (fun r -> HS.is_eternal_region r)
+  (fun _ -> ())
+  b
+  (fun r -> MR.m_recall r)
+  (fun r -> MR.m_read r)
+  (fun l v h0 -> b (MR.m_sel h0 l) v)
+  (fun l v -> MR.m_write l v)
 
-abstract
-let is_mref (l: loc): GTot bool = LocMRef? l
+let mref (r: MR.rid) (a: Type) (b: MR.reln a) : Tot Type =
+  (l: loc { Loc?.cl l == mref_cl r a b } )
 
-abstract
-let is_iseq (l: loc): GTot bool = LocISeq? l
-
-let rid = HH.rid
-let mr_rid = MR.rid
-let ms_rid = MS.rid
-
-// abstract // this is not possible, unification issues
-let loc_region_type (l: loc) : GTot Type =
-  if is_iseq l then ms_rid else
-  if is_mref l then mr_rid else
-  rid
-
-abstract
-let loc_region (l: loc): GTot (loc_region_type l) =
-  match l with
-  | LocRef _ r -> HS.frameOf r
-  | LocMRef r _ _ _ -> r
-  | LocISeq r _ _ _ -> r
-
-let reln = MR.reln
-
-let grows (#a: Type) (#p: (Seq.seq a -> Type)) (s1 s2: guarded (Seq.seq a) p) = MS.grows (s1 <: Seq.seq a) (s2 <: Seq.seq a)
-
+unfold
 let hetero_id
   (to: Type)
   (#from: Type)
@@ -82,222 +107,70 @@ let hetero_id
   (ensures (fun y -> y == x /\ x == y))
 = x
 
-let hetero_id'
-  (to: Type)
-  (#from: Type)
-  (x: from)
-  (q: squash (to == from))
-: Pure to
-  (requires True)
-  (ensures (fun y -> y == x /\ x == y))
-= x
-
-abstract
-let loc_reln (l: loc { is_mref l \/ is_iseq l }) : GTot (reln (loc_type l)) =
-  match l with
-  | LocMRef _ _ b _ -> b
-  | LocISeq _ a p _ -> grows #a #p
-
-abstract
-let loc_mref (l: loc { is_mref l }) : GTot (MR.m_rref (loc_region l) (loc_type l) (loc_reln l)) =
-  LocMRef?.contents l
-
-abstract
-let loc_is_at_most_one
-  (l: loc)
-: Lemma
-  (ensures (
-    (if is_ref l then 1 else 0) +
-    (if is_mref l then 1 else 0) +
-    (if is_iseq l then 1 else 0) <=
-    1
-  ))
-= ()
-
-abstract
-let is_mref_inj
-  (l1: loc {is_mref l1})
-  (l2: loc {is_mref l2})
-: Lemma
-  (requires (loc_region l1 === loc_region l2 /\ loc_type l1 == loc_type l2 /\ loc_reln l1 === loc_reln l2 /\ loc_mref l1 === loc_mref l2))
-  (ensures (l1 == l2))
-= ()
-
-abstract
-let loc_iseq_type
-  (l: loc {is_iseq l})
-: GTot Type
-= LocISeq?.a l
-
-let ref
-  (a: Type)
-: Tot Type
-= (l: loc { is_ref l /\ loc_type l == a } )
-
-let mref
-  (r: MR.rid)
-  (a: Type)
-  (b: MR.reln a)
-: Tot Type
-= (l: loc { is_mref l /\ loc_type l == a /\ loc_region l == r /\ loc_reln l == b } )
-
-let loc_invar
-  (l: loc { is_iseq l } )
-: GTot (Seq.seq (loc_iseq_type l) -> Type)
-= LocISeq?.p l
-
-let iseq
+unfold
+let i_as_hsref
   (r: MS.rid)
   (a: Type)
   (p: (Seq.seq a -> Type))
-: Tot Type
-= (l: (l: loc { is_iseq l } ) { loc_iseq_type l == a /\ loc_region l == r /\ loc_invar l == p } )
+  (x: MS.i_seq r a p)
+: GTot (HS.reference (s: (Seq.seq a) {p s}))
+= let (x : HS.ref (s: Seq.seq a {p s}) { x.HS.id = r}) = MR.as_hsref x in
+  let (y: HS.reference (s: Seq.seq a {p s})) = x in
+  hetero_id (HS.reference (s: Seq.seq a {p s})) y ()
 
-let loc_type_iseq
-  (#r: MS.rid)
-  (#a: Type)
-  (#p: (Seq.seq a -> Type))
-  (x: iseq r a p)
-: Lemma
-  (loc_type x == guarded (Seq.seq a) p)
-  [SMTPat (loc_type x)]
-= ()
+unfold
+let iseq_cl (r: MS.rid) (a: Type) (p: (Seq.seq a -> Type)) : Tot class = Class
+  (MS.i_seq r a p)
+  (s: (Seq.seq a) {p s})
+  (i_as_hsref r a p)
+  (fun r -> HS.is_eternal_region r)
+  (fun _ -> ())
+  (grows a p)
+  (fun r -> MR.m_recall r)
+  (fun r -> MS.i_read r)
+  (fun _ _ _ -> False)
+  (fun _ _ -> ())
 
-let loc_reln_iseq
-  (#r: MS.rid)
-  (#a: Type)
-  (#p: (Seq.seq a -> Type))
-  (x: iseq r a p)
-: Lemma
-  (loc_reln x == grows #a #p)
-  [SMTPat (loc_reln x)]
-= ()
+let iseq (r: MS.rid) (a: Type) (p: (Seq.seq a -> Type)) : Tot Type =
+  (l: loc { Loc?.cl l == iseq_cl r a p } )
 
-abstract
-let ref_of_reference
-  (#a: Type)
-  (r: HS.reference a)
-: GTot (ref a)
-= LocRef a r
+unfold
+let loc_type (l: loc) : Tot Type = Class?.value (Loc?.cl l)
 
-abstract
-let reference_of_ref
-  (#a: Type)
-  (r: ref a)
-: GTot (HS.reference a)
-= loc_ref r
+// unfold  // impossible, makes `loc_region` no longer typecheck
+let loc_region_type (l: loc) : Tot Type =
+  (r: HH.rid { Class?.region_guard (Loc?.cl l) r})
 
-abstract
-let ref_of_reference_of_ref
-  (#a: Type)
-  (r: ref a)
-: Lemma
-  (ref_of_reference (reference_of_ref r) == r)
-= ()
+unfold
+let loc_region (l: loc) : GTot (loc_region_type l) =
+  let (Loc c r) = l in
+  Class?.region_guarded c r;
+  HS.frameOf (Class?.as_reference c r)
 
-abstract
-let reference_of_ref_of_reference
-  (#a: Type)
-  (r: HS.reference a)
-: Lemma
-  (reference_of_ref (ref_of_reference r) == r)
-= ()
+unfold
+let as_reference
+  (l: loc)
+: GTot (HS.reference (loc_type l))
+= Class?.as_reference (Loc?.cl l) (Loc?.obj l)
 
-let mref_of_m_rref
-  (#r: MR.rid)
-  (#a: Type)
-  (#b: MR.reln a)
-  (mr: MR.m_rref r a b)
-: GTot (mref r a b)
-= LocMRef r a b mr
-
-let m_rref_of_mref
-  (#r: MR.rid)
-  (#a: Type)
-  (#b: MR.reln a)
-  (mr: mref r a b)
-: GTot (MR.m_rref r a b)
-= loc_mref mr 
-
-abstract
-let iseq_of_i_seq
-  (#r: MS.rid)
-  (#a: Type)
-  (#p: (Seq.seq a -> Type))
-  (ms: MS.i_seq r a p)
-: GTot (iseq r a p)
-= LocISeq r a p ms
-
-abstract
-let i_seq_of_iseq
-  (#r: MS.rid)
-  (#a: Type)
-  (#p: (Seq.seq a -> Type))
-  (ms: iseq r a p)
-: GTot (MS.i_seq r a p)
-= LocISeq?.contents ms
-
-abstract
+unfold
 let sel
   (h: mem)
   (l: loc)
 : GTot (loc_type l)
-= match l with
-  | LocRef _ rr -> HS.sel h rr
-  | LocMRef _ _ _ rr -> MR.m_sel h rr
-  | LocISeq r a p rr ->
-    let x : guarded (Seq.seq a) p = MS.i_sel h rr in x
-
-abstract
-let as_reference
-  (l: loc)
-: GTot (HS.reference (loc_type l))
-= match l with
-  | LocRef _ rr -> rr
-  | LocMRef _ _ _ rr -> MR.as_hsref rr
-  | LocISeq r a p rr -> 
-    let (x : HS.ref (s: Seq.seq a {p s}) { x.HS.id = r}) = MR.as_hsref rr in
-    let (y: HS.reference (s: Seq.seq a {p s})) = x in
-    assert_norm (guarded (Seq.seq a) p == (s: Seq.seq a {p s}));
-    hetero_id (HS.reference (guarded (Seq.seq a) p)) y ()
-
-private
-let loc_region_iseq
-  r a p x
-: Lemma
-  ((as_reference (LocISeq r a p x)).HS.id == loc_region (LocISeq r a p x))
-  [SMTPatOr [
-    [SMTPat (as_reference (LocISeq r a p x)).HS.id];
-    [SMTPat (loc_region (LocISeq r a p x))];
-  ]]
-= assert ((MR.as_hsref x).HS.id == r) // TODO: WHY WHY WHY not automatic?
+= HS.sel h (as_reference l)
 
 let live_region = HS.live_region
 
-abstract
+unfold
 let upd
   (h: mem)
   (l: loc { live_region h (loc_region l) } )
-  (x: loc_type l)
-: GTot mem
-= match l with
-  | LocRef _ rr -> HS.upd h rr x
-  | LocMRef _ _ _ rr -> HS.upd h (MR.as_hsref rr) x
-  | LocISeq r a p rr ->
-    let x : guarded (Seq.seq a) p = x in
-    HS.upd h (MR.as_hsref rr) x
+  (v: loc_type l)
+: GTot (mem)
+= HS.upd h (as_reference l) v
 
-private
-let upd_iseq
-  (h: mem)
-  (r: MS.rid) a p rr
-  (x: guarded (Seq.seq a) p)
-: Lemma
-  (requires (live_region h r))
-  (ensures (live_region h r /\ upd h (LocISeq r a p rr) x == HS.upd h (MR.as_hsref rr) x))
-  [SMTPat (upd h (LocISeq r a p rr))]
-= assert_norm (upd h (LocISeq r a p rr) x == HS.upd h (MR.as_hsref rr) x)
-
+abstract
 let sel_upd
   (h: mem)
   (l: loc { live_region h (loc_region l) })
@@ -306,6 +179,44 @@ let sel_upd
   (sel (upd h l x) l == x)
   [SMTPat (sel (upd h l x) l)]
 = ()
+
+unfold
+let contains
+  (h: mem)
+  (l: loc)
+= HS.contains h (as_reference l)
+
+let contains_live_region
+  (l: loc)
+  h
+: Lemma
+  (requires (contains h l))
+  (ensures (live_region h (loc_region l)))
+  [SMTPatOr [
+    [SMTPat (contains h l)];
+    [SMTPat (live_region h (loc_region l))];
+  ]]
+= ()
+
+let reln = MR.reln
+
+unfold
+let stable_on_t
+  (l: loc)
+  (p: (mem -> GTot Type0))
+= forall h0 h1 . p h0 /\ Class?.reln (Loc?.cl l) (sel h0 l) (sel h1 l) ==> p h1
+
+let int_at_most #r #a #p (x:int) (is: iseq r a p) (h:mem) : Type0 =
+  let s: Seq.seq a = sel h is in // TODO: WHY WHY WHY is this type cast needed?
+  x < Seq.length s
+
+abstract
+let int_at_most_is_stable (#r:MS.rid) (#a:Type) (#p: Seq.seq a -> Type) (is:iseq r a p) (k:int)
+  : Lemma (ensures (stable_on_t is (int_at_most k is)))
+= assert (forall h . sel h is == MS.i_sel h (Loc?.obj is <: MS.i_seq r a p));
+  MS.int_at_most_is_stable (Loc?.obj is <: MS.i_seq r a p) k
+
+let rid = HH.rid
 
 let modifies_regions
   (rs: Set.set rid)
@@ -441,25 +352,6 @@ let modifies_regions_modifies_locs_in_region
   (ensures (modifies_locs_in_region r TSet.empty h h'))
 = ()
 
-abstract
-let contains
-  (m: mem)
-  (l: loc)
-: Tot Type0
-= HS.contains m (as_reference l)
-
-let contains_live_region
-  (l: loc)
-  h
-: Lemma
-  (requires (contains h l))
-  (ensures (live_region h (loc_region l)))
-  [SMTPatOr [
-    [SMTPat (contains h l)];
-    [SMTPat (live_region h (loc_region l))];
-  ]]
-= ()
-
 let loc_diff
   (l1 l2: loc)
 : GTot Type0
@@ -531,30 +423,20 @@ let mref_not_mm
   (~ (loc_mm m))
 = ()
 
-let is_eternal_region = HS.is_eternal_region
-
-abstract
 let recall
   (l: loc)
 : Stack unit
   (requires (fun _ -> (is_eternal_region (loc_region l) /\ (~ (loc_mm l)))))
   (ensures (fun m0 _ m1 -> m0 == m1 /\ m1 `contains` l))
-= match l with
-  | LocRef a r -> ST.recall r
-  | LocMRef _ _ _ r -> MR.m_recall r
-  | LocISeq _ _ _ r -> MR.m_recall r
+= Class?.recall (Loc?.cl l) (Loc?.obj l)
 
 (* Accessors *)
 
-abstract
 let weak_contains
   (m: mem)
   (l: loc)
 : GTot Type0
 = HS.weak_contains m (as_reference l)
-
-unfold let read_post (r: loc) (m0: mem) (x: loc_type r) (m1: mem) =
-  m1==m0 /\ x==sel m0 r
 
 let weak_live_region = HS.weak_live_region
 
@@ -577,38 +459,47 @@ let weak_contains_mref
   [SMTPat (weak_contains h m)]
 = ()
 
-abstract
+let weak_contains_iseq
+  (#r: MS.rid)
+  (#a: Type)
+  (#p: (Seq.seq a -> Type)) 
+  (m: iseq r a p)
+  (h: mem)
+: Lemma
+  (weak_contains h m)
+  [SMTPat (weak_contains h m)]
+= ()
+
+unfold
+let read_post (r: loc) (m0: mem) (x: loc_type r) (m1: mem) =
+  m1==m0 /\ x==sel m0 r
+
 let read
   (l: loc)
 : ST (loc_type l)
   (requires (fun h -> weak_contains h l))
   (ensures (fun m0 x m1 -> read_post l m0 x m1))
-= match l with
-  | LocRef a r -> !r
-  | LocMRef _ _ _ r -> MR.m_read r
-  | LocISeq i a p r ->
-    let x : guarded (Seq.seq a) p = MS.i_read r in
-    x
+= Class?.read (Loc?.cl l) (Loc?.obj l)
 
-abstract
+unfold
 let write_pre
-  (h0: mem)
   (l: loc)
   (v: loc_type l)
-: GTot Type0
-= match l with
-  | LocRef _ _ -> True
-  | LocMRef _ _ b r -> b (sel h0 l) v
-  | LocISeq _ _ _ _ -> False
+= Class?.write_pre (Loc?.cl l) (Loc?.obj l) v
 
+unfold
+let write_post (r:loc) (v:loc_type r) m0 (_u:unit) m1 =
+  m0 `contains` r /\ m1 == upd m0 r v
+
+(*
 let ref_write_pre
   (#a: Type)
   (h0: mem)
   (r: ref a)
   (v: a)
 : Lemma
-  (write_pre h0 r v)
-  [SMTPat (write_pre h0 r v)]
+  (write_pre r v h0)
+  [SMTPat (write_pre r v h0)]
 = ()
 
 let mref_write_pre
@@ -623,29 +514,15 @@ let mref_write_pre
   (ensures (write_pre h0 m v))
   [SMTPat (write_pre h0 m v)]
 = ()
+*)
 
-let contains_live_region
-  (m0: mem)
-  (l: loc)
-: Lemma
-  (requires (m0 `contains` l))
-  (ensures (live_region m0 (loc_region l)))
-  [SMTPat (live_region m0 (loc_region l))]
-= ()
-
-unfold let write_post (r:loc) (v:loc_type r) m0 (_u:unit) m1 =
-  m0 `contains` r /\ m1 == upd m0 r v
-
-abstract
 let write
   (l: loc)
   (v: loc_type l)
 : ST unit
-  (requires (fun h0 -> h0 `contains` l /\ write_pre h0 l v))
+  (requires (fun h0 -> h0 `contains` l /\ write_pre l v h0))
   (ensures (write_post l v))
-= match l with
-  | LocRef _ r -> r := v
-  | LocMRef _ _ _ r -> MR.m_write r v
+= Class?.write (Loc?.cl l) (Loc?.obj l) v
 
 let get = ST.get
 
@@ -658,9 +535,7 @@ let write_at_end_pre
   (x: a)
   (h: mem)
 : Tot Type0
-= let w : loc_type r = sel h r in
-  let w = hetero_id (guarded (Seq.seq a) p) w () in
-  p (Seq.snoc w x)
+= p (Seq.snoc (sel h r) x)
 
 unfold
 let write_at_end_post
@@ -674,13 +549,10 @@ let write_at_end_post
   (h1: mem)
 : Tot Type0
 = h0 `contains` r /\ (
-    let w : loc_type r = sel h0 r in
-    let w = hetero_id (guarded (Seq.seq a) p) w () in
-    p (Seq.snoc w x) /\ (
-      let s : guarded (Seq.seq a) p = Seq.snoc w x in
-      let s = hetero_id (loc_type r) s () in
-      h1 == upd h0 r s
-  ))
+    let s = Seq.snoc (sel h0 r) x in
+    p s /\
+    h1 == upd h0 r s
+  )
 
 abstract
 let write_at_end
@@ -693,88 +565,9 @@ let write_at_end
   (requires (write_at_end_pre r x))
   (ensures (write_at_end_post r x))
 = recall r;
-  let w : guarded (Seq.seq a) p = read r in
-  let s : guarded (Seq.seq a) p = Seq.snoc w x in
-  let rr = LocISeq?.contents r in
+  let w = read r in
+  let s = Seq.snoc w x in
+  let rr : MS.i_seq rgn a p = Loc?.obj r in
   let h0 = get () in
   assert (h0 `HS.contains` (MR.as_hsref rr));
   MR.m_write rr s
-
-let int_at_most #r #a #p (x:int) (is:iseq r a p) (h:mem) : Type0 =
-  let s : guarded (Seq.seq a) p = sel h is in
-  let s : Seq.seq a = s in
-  x < Seq.length s
-
-private
-let int_at_most_equiv #r #a #p (x:int) (is:iseq r a p) (h:mem)
-: Lemma
-  (int_at_most x is h <==> MS.int_at_most x (LocISeq?.contents is) h)
-  [SMTPat (int_at_most x is h)]
-= ()
-
-unfold let stable_on_t
-  (l: loc { is_mref l \/ is_iseq l } )
-  (p: (mem -> GTot Type0))
-= forall h0 h1 . p h0 /\ loc_reln l (sel h0 l) (sel h1 l) ==> p h1
-
-#reset-options "--z3rlimit 32"
-
-private
-let i_sel_eq
-  (#r: ms_rid) (#a: Type) (#p: (Seq.seq a -> Type)) (rr:MS.i_seq r a p)
-  (h0: mem)
-: Lemma
-  (MS.i_sel h0 rr == MR.m_sel h0 rr)
-= ()
-
-private
-let sel_iseq_i_sel
-  (#r: ms_rid) (#a: Type) (#p: (Seq.seq a -> Type)) (is:iseq r a p)
-  (h0: mem)
-  : Lemma
-  (((sel h0 is <: guarded (Seq.seq a) p) <: Seq.seq a) == MS.i_sel h0 (LocISeq?.contents is))
-= ()
-
-private
-let sel_iseq_m_sel
-  (#r: ms_rid) (#a: Type) (#p: (Seq.seq a -> Type)) (is:iseq r a p)
-  (h0: mem)
-  : Lemma
-  (((sel h0 is <: guarded (Seq.seq a) p) <: Seq.seq a) == MR.m_sel h0 (LocISeq?.contents is))
-= i_sel_eq (LocISeq?.contents is) h0; sel_iseq_i_sel is h0
-
-private
-let stable_on_t_iseq
-  (#r: ms_rid) (#a: Type) (#p: (Seq.seq a -> Type)) (is:iseq r a p)
-  (p': (mem -> GTot Type0))
-: Lemma
-  (stable_on_t is p' <==> MR.stable_on_t (LocISeq?.contents is) p')
-= loc_type_iseq is;
-  let f
-    (h0 h1: mem)
-  : Lemma
-    (requires (stable_on_t is p' /\ p' h0 /\ MS.grows (MR.m_sel h0 (LocISeq?.contents is)) (MR.m_sel h1 (LocISeq?.contents is))))
-    (ensures (p' h1))
-  = 
-    sel_iseq_m_sel is h0;
-    sel_iseq_m_sel is h1;
-    assert (grows #a #p (sel h0 is) (sel h1 is))
-  in
-  let g
-    (h0 h1: mem)
-  : Lemma
-    (requires (MR.stable_on_t (LocISeq?.contents is) p' /\ p' h0 /\ grows #a #p (sel h0 is) (sel h1 is)))
-    (ensures (p' h1))
-  =
-    sel_iseq_m_sel is h0;
-    sel_iseq_m_sel is h1
-  in
-  Classical.forall_intro_2 (let f' (h0: mem) = Classical.move_requires (f h0) in f');
-  Classical.forall_intro_2 (let g' (h0: mem) = Classical.move_requires (g h0) in g')
-
-abstract
-let int_at_most_is_stable (#r:ms_rid) (#a:Type) (#p: Seq.seq a -> Type) (is:iseq r a p) (k:int)
-  : Lemma (ensures (stable_on_t is (int_at_most k is)))
-  = stable_on_t_iseq is (int_at_most k is);
-    MS.int_at_most_is_stable (LocISeq?.contents is) k
-    
